# Z4c

$$
\begin{align}
\Gamma^{k}{}_{ij}
&=\frac{1}{2}\gamma^{kl}(\partial_i\gamma_{jl}+\partial_j\gamma_{li}-\partial_l\gamma_{ij})
\\
&=\frac{1}{2}\tilde\gamma^{kl}
\left[
  (\partial_i\tilde\gamma_{jl}-\partial_i\ln\chi\tilde\gamma_{jl})+
  (\partial_j\tilde\gamma_{li}-\partial_j\ln\chi\tilde\gamma_{li})-
  (\partial_l\tilde\gamma_{ij}-\partial_l\ln\chi\tilde\gamma_{ij})
\right]
\\
&=\tilde\Gamma^k{}_{ij}
-\frac{1}{2}
(\partial_i\ln\chi\delta^k{}_j+\partial_j\ln\chi\delta^k{}_i
-\tilde\gamma_{ij}\tilde\gamma^{kl}\partial_l\ln\chi)
\end{align}
$$
where
$\partial_l\gamma_{ij}=\partial_l(\chi^{-1}\tilde\gamma_{ij})
=\chi^{-1}(\partial_l\tilde{\gamma}_{ij}-\chi^{-1}\partial_l\chi\tilde\gamma_{ij})
=\chi^{-1}(\partial_l\tilde{\gamma}_{ij}-\partial_l\ln\chi\tilde\gamma_{ij})$.
